Fredy.lean
@@ -1,1 +1,3 @@
 import Fredy.Basic
+import Fredy.Capital
+import Fredy.SliceLemma
